ByteBitRelations.v
@@ -1,0 +1,259 @@
+Require Import List. Import ListNotations.
+Require Import Coq.ZArith.BinInt. (* Z *)
+Require Import XorCorrespondence. (* Blist *)
+Require Import Integers.          (* byte *)
+Require Import Coq.Numbers.Natural.Peano.NPeano.
+Require Import HMAC_functional_prog_Z.
+
+Require Import Coq.Strings.Ascii.
+Require Import Coq.Program.Tactics.
+Require Import Bruteforce.
+
+Open Scope Z_scope.
+
+(* ----- Inductive *)
+
+(* In XorCorrespondence *)
+(* Definition asZ (x : bool) : Z := if x then 1 else 0. *)
+
+(*
+Definition convertByteBits (bits : Blist) (byte : Z) : Prop :=
+  exists (b0 b1 b2 b3 b4 b5 b6 b7 : bool),
+   bits = [b0; b1; b2; b3; b4; b5; b6; b7] /\
+   byte =  (1 * (asZ b0) + 2 * (asZ b1) + 4 * (asZ b2) + 8 * (asZ b3)
+         + 16 * (asZ b4) + 32 * (asZ b5) + 64 * (asZ b6) + 128 * (asZ b7)).
+*)
+
+Inductive bytes_bits_lists : Blist -> list Z -> Prop :=
+  | eq_empty : bytes_bits_lists nil nil
+  | eq_cons : forall (bits : Blist) (bytes : list Z)
+                     (b0 b1 b2 b3 b4 b5 b6 b7 : bool) (byte : Z),
+                bytes_bits_lists bits bytes ->
+                convertByteBits [b0; b1; b2; b3; b4; b5; b6; b7] byte ->
+                bytes_bits_lists (b0 :: b1 :: b2 :: b3 :: b4 :: b5 :: b6 :: b7 :: bits)
+                                 (byte :: bytes).
+
+Definition byte_to_64list (byte : byte) : list Z :=
+   map Byte.unsigned (HMAC_SHA256.sixtyfour byte).
+
+Definition Z_to_64list (num : Z) : list Z :=
+   HMAC_SHA256.sixtyfour num.
+
+(* ----- Computational *)
+
+(* TODO: assumes Z is positive and in range, does not use Z.positive *)
+
+Definition div_mod (num : Z) (denom : Z) : bool * Z :=
+  (Z.gtb (num / denom) 0, num mod denom).
+
+Eval compute in div_mod 129 128.
+Eval compute in div_mod 1 64.
+
+Definition byteToBits (byte : Z) : Blist :=
+  let (b7, rem7) := div_mod byte 128 in
+  let (b6, rem6) := div_mod rem7 64 in
+  let (b5, rem5) := div_mod rem6 32 in
+  let (b4, rem4) := div_mod rem5 16 in
+  let (b3, rem3) := div_mod rem4 8 in
+  let (b2, rem2) := div_mod rem3 4 in
+  let (b1, rem1) := div_mod rem2 2 in
+  let (b0, rem0) := div_mod rem1 1 in
+  [b0; b1; b2; b3; b4; b5; b6; b7].
+
+Fixpoint bytesToBits (bytes : list Z) : Blist :=
+  match bytes with
+    | [] => []
+    | byte :: xs => byteToBits byte ++ bytesToBits xs
+  end.
+
+Definition bitsToByte (bits : Blist) : Z :=
+  match bits with
+    | b0 :: b1 :: b2 :: b3 :: b4 :: b5 :: b6 :: b7 :: nil =>
+      1 * (asZ b0) + 2 * (asZ b1) + 4 * (asZ b2) + 8 * (asZ b3)
+      + 16 * (asZ b4) + 32 * (asZ b5) + 64 * (asZ b6) + 128 * (asZ b7)
+    | _ => -1                   (* should not happen *)
+  end.
+
+Fixpoint bitsToBytes (bits : Blist) : list Z :=
+  match bits with
+    | b0 :: b1 :: b2 :: b3 :: b4 :: b5 :: b6 :: b7 :: xs =>
+      bitsToByte [b0; b1; b2; b3; b4; b5; b6; b7] :: bitsToBytes xs
+    | _ => []
+  end.
+
+Fixpoint bitsToBytes' (bits : Blist) : list Z :=
+  match bits with
+    | b0 :: b1 :: b2 :: b3 :: b4 :: b5 :: b6 :: b7 :: xs =>
+      let byte := 1 * (asZ b0) + 2 * (asZ b1) + 4 * (asZ b2) + 8 * (asZ b3)
+         + 16 * (asZ b4) + 32 * (asZ b5) + 64 * (asZ b6) + 128 * (asZ b7) in
+      byte :: bitsToBytes xs
+    | _ => []
+  end.
+
+(* -------------------- Various theorems and lemmas *)
+
+Lemma bytes_bits_length : forall (bits : Blist) (bytes : list Z),
+  bytes_bits_lists bits bytes -> length bits = (length bytes * 8)%nat.
+Proof.
+  intros bits bytes corr.
+  induction corr.
+  - reflexivity.
+  - simpl. repeat f_equal. apply IHcorr.
+Qed.
+
+Lemma bytesToBits_app : forall (l1 l2 : list Z),
+                          bytesToBits (l1 ++ l2) = bytesToBits l1 ++ bytesToBits l2.
+Proof.
+  induction l1; intros.
+  * reflexivity.
+  *
+    simpl. rewrite -> IHl1. reflexivity.
+Qed.    
+
+Lemma bytesToBits_len : forall (l : list Z),
+                          length (bytesToBits l) = (length l * 8)%nat.
+Proof.
+  induction l; intros; try reflexivity.
+  -
+    simpl.
+    rewrite -> IHl.
+    reflexivity.
+Qed.    
+
+(* Prove by brute force (test all Z in range) *)
+Theorem byte_bit_byte_id : forall (byte : Z),
+                             0 <= byte < 256 ->
+                                bitsToByte (byteToBits byte) = byte.
+Proof.
+  intros byte range.
+  do_range range reflexivity.
+Qed.
+(* TODO move this into a different file; takes a while to check *)
+
+Theorem bits_byte_bits_id : forall (b0 b1 b2 b3 b4 b5 b6 b7 : bool),
+                              [b0; b1; b2; b3; b4; b5; b6; b7] =
+                              byteToBits (bitsToByte [b0; b1; b2; b3; b4; b5; b6; b7]).
+Proof.
+  intros.
+  destruct b0; destruct b1; destruct b2; destruct b3;
+  destruct b4; destruct b5; destruct b6; destruct b7;
+  reflexivity.
+Qed.
+
+Theorem bytes_bits_bytes_id : forall (bytes : list Z),
+                                Forall (fun b => 0 <= b < 256) bytes ->
+                                bitsToBytes (bytesToBits bytes) = bytes.
+Proof.
+  intros range bytes.
+  induction bytes as [ | byte bytes].
+  - reflexivity.
+  -
+    unfold bytesToBits.
+    fold bytesToBits.
+    unfold byteToBits.
+    unfold bitsToBytes.
+    Opaque bitsToByte. Opaque bitsToBytes. Opaque bytesToBits.
+    simpl.
+    Transparent bitsToBytes. fold bitsToBytes.
+    rewrite -> IHbytes.
+    
+    Transparent bitsToByte.
+    unfold bitsToByte. f_equal.
+    apply byte_bit_byte_id.
+    
+    apply H. Transparent bytesToBits.
+Qed.
+
+Close Scope string_scope.
+
+(* ------------------ Theorems relating inductive and computational definitions *)
+
+Theorem bytes_bits_def_eq : forall (bytes : list Z),
+                              Forall (fun b => 0 <= b < 256) bytes ->
+                              bytes_bits_lists (bytesToBits bytes) bytes.
+Proof.
+  intros range bytes.
+  induction bytes as [ | byte bytes ].
+  -
+    simpl. apply eq_empty.
+  -
+    apply eq_cons.
+
+    *
+      apply IHbytes.
+    *
+      unfold convertByteBits.
+      do 8 eexists.
+      split.
+      +
+        reflexivity.
+      +
+        do_range H reflexivity.
+Qed.
+
+Theorem bytes_bits_comp_ind : forall (bits : Blist) (bytes : list Z),
+                               Forall (fun b => 0 <= b < 256) bytes ->
+                               bits = bytesToBits bytes ->
+                               bytes_bits_lists bits bytes.
+Proof.
+  intros bits bytes range corr.
+  rewrite -> corr.
+  apply bytes_bits_def_eq.
+  assumption.
+Qed.
+
+Theorem bytes_bits_ind_comp : forall (bits : Blist) (bytes : list Z),
+                                 Forall (fun b => 0 <= b < 256) bytes ->
+                                 bytes_bits_lists bits bytes ->
+                                 bytes = bitsToBytes bits.
+Proof.
+  intros bits bytes range corr.
+  induction corr.
+  - reflexivity.
+  -
+    rewrite -> IHcorr.
+    *
+      unfold convertByteBits in H.
+      unfold bitsToBytes.
+      fold bitsToBytes.
+      f_equal.
+
+      assert (range' : 0 <= byte < 256). admit.
+
+      unfold bitsToByte.
+      Print convertByteBits.
+      destruct_exists. destruct H7. inversion H7.
+      subst. reflexivity.
+
+      * admit.                  (* bytes in range *)
+Qed.
+
+Theorem bits_bytes_ind_comp : forall (bits : Blist) (bytes : list Z),
+                                 Forall (fun b => 0 <= b < 256) bytes ->
+                                 bytes_bits_lists bits bytes ->
+                                 bits = bytesToBits bytes.
+Proof.
+  intros bits bytes range corr.
+  induction corr.
+  - reflexivity.
+  -
+    unfold convertByteBits in H.
+    destruct_exists.
+    destruct H7.
+    inversion H7.
+    subst.
+    clear H7.
+    rewrite -> IHcorr.
+    unfold bytesToBits.
+    fold bytesToBits.
+    assert (list_8 : forall {A : Type} (e0 e1 e2 e3 e4 e5 e6 e7 : A) (l : list A),
+                       e0 :: e1 :: e2 :: e3 :: e4 :: e5 :: e6 :: e7 :: l =
+                       [e0; e1; e2; e3; e4; e5; e6; e7] ++ l).
+    reflexivity.
+    rewrite -> list_8.
+    f_equal.
+    apply bits_byte_bits_id.
+
+    admit.                      (* in range *)
+Qed.
+    
