HMAC_spec_list.v
@@ -1,0 +1,79 @@
+Set Implicit Arguments.
+
+
+Require Import Bvector.
+Require Import List.
+Require Import Arith.
+
+Definition Blist := list bool.
+
+Fixpoint splitVector(A : Set)(n m : nat) : Vector.t A (n + m) -> (Vector.t A n * Vector.t A m) :=
+  match n with
+    | 0 => 
+      fun (v : Vector.t A (O + m)) => (@Vector.nil A, v)
+    | S n' => 
+      fun (v : Vector.t A (S n' + m)) => 
+        let (v1, v2) := splitVector _ _ (Vector.tl v) in
+          (Vector.cons _ (Vector.hd v) _ v1, v2)
+  end.
+
+(* TODO: forces n + m = length of input, should really take one parameter (n) *)
+Eval compute in splitVector 1 2 [1;2;3].
+
+(* TODO: revise this to take only n? *)
+Definition splitList {A : Type} (h : nat) (t : nat) (l : list A) : (list A * list A) :=
+  (firstn h l, skipn t l).
+
+Section HMAC.
+
+  Variable c p : nat.
+  Definition b := c + p.
+  
+  (* The compression function *)
+  Variable h : Blist -> Blist -> Blist.
+  (* The initialization vector is part of the spec of the hash function. *)
+  Variable iv : Blist.
+  (* The iteration of the compression function gives a keyed hash function on lists of words. *)
+  Definition h_star k (m : list (Blist)) :=
+    fold_left h m k.
+  (* The composition of the keyed hash function with the IV gives a hash function on lists of words. *)
+  Definition hash_words := h_star iv.
+
+  Variable splitAndPad : Blist -> list (Blist).
+  Hypothesis splitAndPad_1_1 : 
+    forall b1 b2,
+      splitAndPad b1 = splitAndPad b2 ->
+      b1 = b2.
+
+  (* fpad can be a constant *)
+  Variable fpad : Blist -> Blist. 
+  Definition app_fpad (x : Blist) : Blist :=
+    x ++ fpad x.
+
+  Definition h_star_pad k x :=
+    app_fpad (h_star k x).
+
+  Definition GNMAC k m :=
+    let (k_Out, k_In) := splitVector c c k in
+    h k_Out (app_fpad (h_star k_In m)).
+
+  (* The "two-key" version of GHMAC and HMAC. *)
+  Definition GHMAC_2K (k : Bvector (b + b)) m :=
+    let (k_Out, k_In) := splitVector b b k in
+      let h_in := (hash_words (k_In :: m)) in 
+        hash_words (k_Out :: (app_fpad h_in) :: nil).
+  
+  Definition HMAC_2K (k : Bvector (b + b)) (m : Blist) :=
+    GHMAC_2K k (splitAndPad m).
+
+  (* opad and ipad are constants defined in the HMAC spec. *)
+  Variable opad ipad : Blist.
+  Hypothesis opad_ne_ipad : opad <> ipad.
+
+  Definition GHMAC (k : Blist) :=
+    GHMAC_2K (Vector.append (BVxor _ k opad) (BVxor _ k ipad)).
+
+  Definition HMAC (k : Blist) :=
+    HMAC_2K (Vector.append (BVxor _ k opad) (BVxor _ k ipad)).
+
+End HMAC.
